ML_SP_Inference.v
@@ -1,0 +1,598 @@
+(***************************************************************************
+* Principality of type inference for mini-ML with structural polymorphism  *
+* Jacques Garrigue, August 2008                                            *
+***************************************************************************)
+
+Set Implicit Arguments.
+
+Require Import List Metatheory.
+
+Section Index.
+  Variable A : Set.
+  Hypothesis eq_dec : forall x y : A, {x = y}+{x <> y}.
+
+  Fixpoint index (i:nat) (x:A) (l : list A) {struct l} : option nat :=
+    match l with
+    | nil   => None
+    | y::l' => if eq_dec x y then Some i else index (S i) x l'
+    end.
+End Index.
+
+Require Import ML_SP_Definitions ML_SP_Infrastructure.
+Require Import ML_SP_Soundness ML_SP_Unify.
+
+Module MkInfer(Cstr:CstrIntf)(Const:CstIntf).
+
+Module Unify := MkUnify(Cstr)(Const).
+Import Unify.
+Import Sound0.Infra.
+Import Defs.
+Import Metatheory_Env.Env.
+
+Module Mk2(Delta:DeltaIntf)(Cstr2:Cstr2I).
+
+Module Sound := Sound0.Mk2(Delta).
+Import Sound.
+Import JudgInfra.
+Import Judge.
+
+Module Body := Unify.Mk2(Cstr2).
+Import Body.
+
+Definition unify K T1 T2 S :=
+  unify (1 + size_pairs S K ((T1,T2)::nil)) ((T1,T2)::nil) K S.
+
+Definition fvs S K E T :=
+  dom S \u fv_in typ_fv S \u dom K \u fv_in kind_fv K \u env_fv E \u typ_fv T.
+
+Definition close_fvk K := close_fvars (length K) K (dom K).
+
+Fixpoint generalize (Bs:list var) (T:typ) {struct T} : typ :=
+  match T with
+  | typ_bvar n =>
+    typ_bvar (length Bs + n)
+  | typ_fvar x =>
+    match index eq_var_dec 0 x Bs with
+    | None   => T
+    | Some n => typ_bvar n
+    end
+  | typ_arrow T1 T2 =>
+    typ_arrow (generalize Bs T1) (generalize Bs T2)
+  end.
+
+Fixpoint split_env (A:Set) (B:vars) (E:env A) {struct E} : env A * env A :=
+  match E with
+  | nil => (nil, nil)
+  | xk::E' =>
+    let (Eb, EB) := split_env B E' in
+    if S.mem (fst xk) B then (Eb, xk::EB) else (xk::Eb, EB)
+  end.
+
+Fixpoint typinf (K:kenv) (E:Defs.env) (t:trm) (T:typ) (S:subs) (h:nat)
+  {struct h} : option (kenv * subs) :=
+  match h with
+  | 0 => None
+  | S h' =>
+  match t with
+  | trm_bvar _ => None
+  | trm_fvar x =>
+    match get x E with
+    | None => None
+    | Some M =>
+      let Vs := proj1_sig (var_freshes (fvs S K E T) (sch_arity M)) in
+      unify (K & kinds_open_vars (sch_kinds M) Vs) (M ^ Vs) T S
+    end
+  | trm_abs t1 =>
+    let x := proj1_sig (var_fresh (dom E \u trm_fv t1)) in
+    let v1 := proj1_sig (var_fresh (fvs S K E T)) in
+    let V2 := typ_fvar (proj1_sig (var_fresh (fvs S K E T \u {{v1}}))) in
+    match unify K (typ_arrow (typ_fvar v1) V2) T S with
+    | None => None
+    | Some (K',S') =>
+      typinf K' (E & x ~ Sch (typ_fvar v1) nil) (t1 ^ x) V2 S' h'
+    end
+  | trm_let t1 t2 =>
+    let V := typ_fvar (proj1_sig (var_fresh (fvs S K E T))) in
+    match typinf K E t1 V S h' with
+    | None => None
+    | Some (K0,S') =>
+      let K' := Env.map (kind_subst S') K0 in
+      let E' := Env.map (sch_subst S') E in
+      let ftve := close_fvk K (env_fv E') in
+      let T1 := typ_subst S' V in
+      let B := close_fvk K (S.diff (typ_fv T1) ftve) in
+      let (Kb, KB) := split_env B K in
+      let (Bs, Ks) := split KB in
+      let x := proj1_sig (var_fresh (dom E \u trm_fv t1 \u trm_fv t2)) in
+      typinf Kb
+        (E & x~Sch (generalize Bs T1) (List.map (kind_map (generalize Bs)) Ks))
+        (t2 ^ x) T S' h'
+    end
+  | trm_app t1 t2 =>
+    let V := typ_fvar (proj1_sig (var_fresh (fvs S K E T))) in
+    match typinf K E t1 (typ_arrow V T) S h' with
+    | None => None
+    | Some (K',S') => typinf K' E t2 V S' h'
+    end
+  | trm_cst c =>
+    let M := Delta.type c in
+    let Vs := proj1_sig (var_freshes (fvs S K E T) (sch_arity M)) in
+    unify (K & kinds_open_vars (sch_kinds M) Vs) (M ^ Vs) T S
+  end
+  end.
+
+Fixpoint trm_depth (t : trm) : nat :=
+  match t with
+  | trm_bvar _ => 0
+  | trm_fvar _ => 0
+  | trm_abs t1 => S (trm_depth t1)
+  | trm_let t1 t2 => S (Max.max (trm_depth t1) (trm_depth t2))
+  | trm_app t1 t2 => S (Max.max (trm_depth t1) (trm_depth t2))
+  | trm_cst _ => 0
+  end.
+
+Lemma env_prop_type_compose : forall S1 S2,
+  env_prop type S1 -> env_prop type S2 -> env_prop type (compose S1 S2).
+Proof.
+  unfold compose.
+  intros.
+  intro; intros.
+  binds_cases H1.
+    destruct (binds_map_inv _ _ B) as [T [Eq B']].
+    subst.
+    apply* typ_subst_type.
+  auto*.
+Qed.
+
+Section EnvProp.
+  Variables (A:Set) (P:A->Prop).
+
+  Lemma env_prop_single : forall x a, P a -> env_prop P (x ~ a).
+  Proof.
+    intros; intro; intros.
+    destruct (binds_single_inv H0). subst*.
+  Qed.
+
+  Lemma env_prop_concat : forall l1 l2,
+    env_prop P l1 -> env_prop P l2 -> env_prop P (l1 & l2).
+  Proof.
+    intros; intro; intros.
+    binds_cases H1. apply* (H x).
+    apply* (H0 x).
+  Qed.
+
+End EnvProp.
+
+Hint Resolve env_prop_single env_prop_concat env_prop_type_compose.
+
+Lemma For_all_app : forall (A:Set) (P:A->Prop) l1 l2,
+  For_all P l1 -> For_all P l2 -> For_all P (l1++l2).
+Proof.
+  intros; induction l1. simpl*.
+  simpl in *.
+  auto*.
+Qed.
+
+Lemma unify_rel_all_kind_types :
+  forall (P:typ->Prop) k k0 kc (v1:Cstr.valid kc),
+  All_kind_types P (Some k) -> All_kind_types P (Some k0) ->
+  let krs := kind_rel k ++ kind_rel k0 in
+  All_kind_types P (Some (Kind v1 (unify_coherent krs))) /\
+  (forall T1 T2,
+   In (T1, T2) (snd (unify_kind_rel krs nil (Cstr2.unique kc) nil)) ->
+   P T1 /\ P T2).
+Proof.
+  unfold All_kind_types; intros.
+  simpl in *.
+  use (For_all_app _ _ _ H H0).
+  clear H H0.
+  rewrite <- map_app in H1.
+  set (kr':=@nil (var*typ)).
+  set (pairs':=@nil (typ*typ)).
+  assert (For_all P (List.map (fun x : var * typ => snd x) kr')) by simpl*.
+  assert (forall T1 T2, In (T1, T2) pairs' -> P T1 /\ P T2) by simpl*.
+  gen kr' pairs'.
+  induction (kind_rel k ++ kind_rel k0); simpl; intros. auto.
+  destruct a.
+  simpl in H1.
+  destruct (In_dec eq_var_dec v (Cstr2.unique kc)).
+    case_eq (get v kr'); intros.
+      apply* IHl.
+      simpl; intros.
+      destruct* H3.
+      inversions H3.
+      split*.
+      clear -H H2.
+      induction kr'; simpl in *. discriminate.
+      destruct a. destruct (v == v0).
+        inversions* H2.
+      apply* IHkr'.
+    apply* IHl.
+    simpl*.
+  apply* IHl.
+  simpl*.
+Qed.
+
+Lemma kenv_ok_remove_env : forall K v,
+  kenv_ok K -> kenv_ok (remove_env K v).
+Proof.
+  intros; split*.
+  intro; intros.
+  apply (proj2 H x).
+  apply* binds_orig_remove_env.
+Qed.
+
+Hint Resolve kenv_ok_remove_env.
+
+Lemma All_kind_types_None : forall P, All_kind_types P None.
+Proof.
+  unfold All_kind_types. simpl*.
+Qed.
+
+Hint Resolve All_kind_types_None.
+
+Lemma unify_type : forall K' S' h pairs K S,
+  Body.unify h pairs K S = Some (K', S') ->
+  is_subst S ->
+  env_prop type S ->
+  kenv_ok K ->
+  (forall T1 T2, In (T1, T2) pairs -> type T1 /\ type T2) ->
+  kenv_ok K' /\ env_prop type S'.
+Proof.
+  induction h; simpl; intros. discriminate.
+  destruct pairs. inversions* H.
+  destruct p.
+  assert (type t /\ type t0). apply* H3.
+  destruct H4.
+  use (typ_subst_type H1 H4).
+  use (typ_subst_type H1 H5).
+  case_rewrite (typ_subst S t) R1; try solve [inversion H6];
+    case_rewrite (typ_subst S t0) R2; try solve [inversion H7];
+      try (unfold unify_nv in H;
+           case_rewrite (S.mem v (typ_fv (typ_arrow t1 t2))) R3;
+           case_rewrite (get_kind v K) R4; apply* IHh).
+    destruct (v == v0). apply* IHh.
+    unfold unify_vars in H.
+    assert (Hok: forall k, ok (remove_env (remove_env K v) v0 & v0 ~ k)).
+      intro; constructor.
+      repeat apply* ok_remove_env.
+      rewrite* dom_remove_env.
+    assert (Horig: forall x a,
+      binds x a (remove_env (remove_env K v) v0) -> All_kind_types type a).
+      intros; apply (proj2 H2 x a).
+      use (binds_orig_remove_env v0 (ok_remove_env v (proj1 H2)) H8).
+      apply* binds_orig_remove_env.
+    case_rewrite (get_kind v K) R3; case_rewrite (get_kind v0 K) R4;
+      try poses Aktc (proj2 H2 _ _ (get_kind_binds _ _ R3));
+      try poses Aktc0 (proj2 H2 _ _ (get_kind_binds _ _ R4));
+      simpl unify_kinds in H.
+          destruct c as [kc kv kr kh].
+          destruct c0 as [kc0 kv0 kr0 kh0].
+          destruct (Cstr2.valid (Cstr2.lub kc kc0)); try discriminate.
+          replace kr with (kind_rel (Kind kv kh)) in H by simpl*.
+          replace kr0 with (kind_rel (Kind kv0 kh0)) in H by simpl*.
+          destruct*
+            (unify_rel_all_kind_types type (Kind kv kh) (Kind kv0 kh0) v1).
+          apply* IHh; clear IHh H.
+          split*.
+          intros.
+          destruct* (in_app_or _ _ _ H).
+        destruct c as [kc kv kr kh].
+        simpl app in H.
+        apply* IHh. split*.
+      cbv iota beta in H. simpl app in H.
+      apply* IHh. split*.
+    cbv iota beta in H. simpl app in H.
+    apply* IHh. split*.
+  apply* IHh; clear IHh H.
+  simpl; intros.
+  inversions H6.
+  inversions H7.
+  destruct H. inversions* H.
+  destruct H. inversions* H.
+  apply* H3.
+Qed.
+
+Lemma concat_empty_l : forall (A:Set) (E:env A),
+  empty & E = E.
+Proof.
+  unfold concat, empty. intros; rewrite* <- app_nil_end.
+Qed.
+
+Lemma env_incl_map : forall (A:Set) (f:A->A) E1 E2,
+  env_incl E1 E2 -> env_incl (map f E1) (map f E2).
+Proof.
+  intros; intro; intros.
+  destruct (binds_map_inv _ _ H0) as [a [HE B]].
+  subst.
+  apply* binds_map.
+Qed.
+Lemma split_env_ok : forall (A:Set) (B:vars) (E Eb EB:env A),
+  split_env B E = (Eb, EB) -> ok E ->
+  ok (Eb & EB) /\ disjoint B (dom Eb) /\ dom EB << B /\
+  env_incl E (Eb & EB) /\ env_incl (Eb & EB) E.
+Proof.
+  induction E; simpl; intros.
+    inversions H. simpl. split*. split. intro; auto*.
+    split. intros x Hx. elim (in_empty Hx).
+    assert (env_incl (A:=A) nil nil) by (intro; tauto).
+    auto.
+  destruct a.
+  case_rewrite (split_env B E) R1.
+  simpl in *.
+  case_rewrite (S.mem v B) R2.
+    inversions H; clear H.
+    inversions H0; clear H0.
+    destruct* (IHE Eb e0) as [Hok [Dis [Dom [I1 I2]]]]; clear IHE.
+    destruct (ok_concat_inv _ _ Hok).
+    case_eq (get v (Eb & e0)); intros.
+      elim (binds_fresh (I2 _ _ H1) H4).
+    poses Hv' (get_none_notin _ H1); clear H1.
+    split.
+      apply* disjoint_ok.
+        apply* (@ok_push _ e0 v a).
+      use (ok_disjoint _ _ Hok).
+      simpl.
+      disjoint_solve.
+      destruct* (v0 == v). subst*.
+    split*.
+    split.
+      simpl. intros x Hx. destruct* (S.union_1 Hx).
+      rewrite <- (S.singleton_1 H1).
+      apply* S.mem_2.
+    replace ((v,a) :: E) with (E & v ~ a) by simpl*.
+    replace ((v,a) :: e0) with (e0 & v ~ a) by simpl*.
+    split; intro; intros; binds_cases H1; auto*.
+  inversions H; clear H.
+  inversions H0; clear H0.
+  destruct* (IHE e EB) as [Hok [Dis [Dom [I1 I2]]]]; clear IHE.
+  destruct (ok_concat_inv _ _ Hok).
+  case_eq (get v (e & EB)); intros.
+    elim (binds_fresh (I2 _ _ H1) H4).
+  poses Hv' (get_none_notin _ H1); clear H1.
+  split.
+    apply* disjoint_ok.
+      apply* (@ok_push _ e v a).
+    use (ok_disjoint _ _ Hok).
+    simpl.
+    disjoint_solve; destruct* (v0 == v). subst*.
+  split.
+    simpl.
+    disjoint_solve; destruct* (v0 == v); subst*.
+  split*.
+  replace ((v,a) :: E) with (E & v ~ a) by simpl*.
+  replace ((v,a) :: e) with (e & v ~ a) by simpl*.
+  split; intro; intros; binds_cases H1; auto*.
+  use (I1 _ _ B0).
+  binds_cases H1; auto*.
+Qed.
+
+Lemma proper_instance_well_subst : forall S K K' M Us,
+  env_prop type S ->
+  well_subst K K' S ->
+  kenv_ok K' ->
+  proper_instance K M Us ->
+  proper_instance K' (sch_subst S M) (List.map (typ_subst S) Us).
+Proof.
+  intros.
+  destruct H2 as [HUs [HM HW]].
+  split.
+    unfold sch_arity; simpl.
+    destruct HUs.
+    split. repeat rewrite map_length. auto.
+    clear -H H3.
+    induction H3; simpl*.
+  split.
+    apply* sch_subst_type.
+  pose (Ts := Us).
+  assert (Us = Ts) by simpl*. clearbody Ts.
+  pattern Us at 2.
+  pattern Us at 2 in HW.
+  rewrite H2 in *.
+  clear H2 HM.
+  destruct M as [T Ks]; unfold sch_arity in *; simpl in *.
+  destruct HUs.
+  gen Ks; induction H3; destruct Ks; simpl; intros; try discriminate. auto.
+  split*.
+  destruct HW.
+  clear IHlist_forall H6.
+  rewrite* <- kind_subst_open.
+  apply* well_kinded_subst.
+Qed.
+
+Lemma All_kind_types_subst : forall k S,
+  All_kind_types type k ->
+  env_prop type S -> All_kind_types type (kind_subst S k).
+Proof.
+  intros; unfold kind_subst; apply All_kind_types_map.
+  apply* All_kind_types_imp.
+Qed.
+
+Lemma kenv_ok_map : forall K S,
+  kenv_ok K -> env_prop type S -> kenv_ok (map (kind_subst S) K).
+Proof.
+  intros.
+  split. apply* ok_map0.
+  destruct H.
+  intro; intros.
+  destruct (binds_map_inv _ _ H2) as [b [Hb B]].
+  subst.
+  apply* All_kind_types_subst.
+Qed.
+
+Lemma kenv_ok_subst : forall K' K Ks Ys S,
+  env_prop type S ->
+  kenv_ok (K & kinds_open_vars Ks Ys) ->
+  kenv_ok K' ->
+  fresh (dom K') (length Ks) Ys ->
+  kenv_ok (K' & map (kind_subst S) (kinds_open_vars Ks Ys)).
+Proof.
+  introv TS HK HK' Fr.
+  apply* kenv_ok_concat.
+    destruct (kenv_ok_concat_inv _ _ HK).
+    apply* kenv_ok_map.
+  rewrite dom_map. rewrite* dom_kinds_open_vars.
+  apply disjoint_comm. apply* (fresh_disjoint (length Ks)).
+Qed.
+
+Lemma well_subst_extend : forall K S K' Ks Ys,
+  env_prop type S ->
+  well_subst K K' S ->
+  fresh (dom S \u dom K') (length Ks) Ys ->
+  well_subst (K & kinds_open_vars Ks Ys)
+     (K' & map (kind_subst S) (kinds_open_vars Ks Ys)) S.
+Proof.
+  introv TS WS Fr.
+  intro; intros.
+  binds_cases H.
+    use (WS _ _ B).
+    inversions H. apply wk_any.
+    simpl. rewrite <- H1.
+    eapply wk_kind.
+      apply binds_concat_fresh. apply H3.
+      rewrite dom_map.
+      unfold kinds_open_vars.
+      apply* notin_combine_fresh.
+      assert (x \in dom K'). apply* binds_dom.
+      auto with sets.
+    auto.
+  rewrite typ_subst_fresh.
+    destruct k as [[kc kv kr kh]|]; try apply wk_any.
+    simpl.
+    eapply wk_kind.
+      apply binds_prepend.
+      use (binds_map (kind_subst S) B0). simpl in H; apply H.
+    apply entails_refl.
+  simpl.
+  intro v; destruct* (v == Z).
+  subst; left.
+  use (binds_dom B0).
+  rewrite dom_kinds_open_vars in H; auto.
+  destruct* (fresh_disjoint _ _ _ Fr Z).
+Qed.
+
+Lemma typing_typ_well_subst : forall gc S K K' E t T,
+  env_prop type S ->
+  well_subst K K' S ->
+  kenv_ok K' ->
+  K ; E |gc|= t ~: T -> 
+  K'; map (sch_subst S) E |gc|= t ~: (typ_subst S T).
+Proof.
+  introv TS WS HK' Typ.
+  gen K'; induction Typ; intros.
+  (* Var *)
+  rewrite~ sch_subst_open. apply* typing_var.
+  apply* proper_instance_well_subst.
+  (* Abs *)
+  simpl.
+  apply_fresh* (@typing_abs gc) as y.
+  replace (Sch (typ_subst S U) nil) with (sch_subst S (Sch U nil)) by auto.
+  assert (y \notin L) by auto.
+  use (H1 _ H2 _ WS HK').
+  (* Let *)
+  apply_fresh* (@typing_let gc (sch_subst S M)
+    (L1 \u dom S \u fv_in typ_fv S \u sch_fv M \u dom K \u dom K')) as y.
+    clear H1 H2. clear L2 T2 t2.
+    simpl. intros Ys Fr.
+    destruct M as [T Ks]. unfold sch_arity in *; simpl in *.
+    rewrite map_length in Fr.
+    assert (HK: kenv_ok (K & kinds_open_vars Ks Ys)).
+      assert (fresh L1 (length Ks) Ys) by auto*.
+      use (H _ H1).
+    rewrite* <- sch_subst_open_vars.
+    rewrite* <- kinds_subst_open_vars.
+    apply* H0; clear H H0.
+      apply* well_subst_extend.
+    apply* kenv_ok_subst.
+  replace (y ~ sch_subst S M) with (map (sch_subst S) (y ~ M)) by simpl*.
+  rewrite <- map_concat.
+  apply* H2.
+  (* App *)
+  simpl in IHTyp1; auto*.
+  (* Cst *)
+  rewrite* sch_subst_open.
+  assert (disjoint (dom S) (sch_fv (Delta.type c))).
+    intro x. rewrite* Delta.closed.
+  rewrite* sch_subst_fresh.
+  apply* typing_cst.
+  rewrite* <- (sch_subst_fresh _ H2).
+  apply* proper_instance_well_subst.
+  (* GC *)
+  apply* (@typing_gc gc (List.map (kind_subst S) Ks)
+                     (L \u dom S \u dom K \u dom K')).
+  rewrite map_length; intros.
+  rewrite* <- kinds_subst_open_vars.
+  apply* (H1 Xs); clear H1.
+    apply* well_subst_extend.
+  forward~ (H0 Xs); intro Typ.
+  apply* (@kenv_ok_subst K' K).
+Qed.
+
+Theorem soundness : forall t h K0 E T S0 K S gc,
+  is_subst S0 -> env_prop type S0 -> kenv_ok K0 ->
+  disjoint (dom S0) (dom K0) ->
+  ok E -> env_prop scheme E -> type T ->
+  typinf K0 E t T S0 h = Some (K, S) ->
+  well_subst (map (kind_subst S0) K0) (map (kind_subst S) K) S /\
+  map (kind_subst S) K; map (sch_subst S) E |gc|= t ~: typ_subst S T.
+Proof.
+  induction t; destruct h; simpl; intros until gc;
+    intros HS0 HTS0 HK0 Dis HE HSE HT HI; try discriminate.
+      case_rewrite (get v E) R1.
+      destruct (var_freshes (fvs S0 K0 E T) (sch_arity s)).
+      simpl proj1_sig in HI.
+      unfold unify in HI.
+      assert (kenv_ok (K0 & kinds_open_vars (sch_kinds s) x)).
+        split.
+          apply* disjoint_ok. unfold kinds_open_vars, kinds_open.
+            apply* ok_combine_fresh.
+          rewrite* dom_kinds_open_vars.
+          unfold fvs in f. disjoint_solve.
+        apply env_prop_concat. apply (proj2 HK0).
+        destruct* (HSE _ _ R1 x).
+        unfold kinds_open_vars, kinds_open.
+        apply list_forall_env_prop.
+        clear -H0; induction (sch_kinds s). simpl*.
+        simpl in *.
+        inversions H0; clear H0.
+        constructor; auto.
+        unfold kind_open. unfold typ_open_vars in H3.
+        apply* All_kind_types_map.
+      destruct* (unify_kinds_ok _ _ HI HS0).
+        unfold fvs in f. rewrite dom_concat. rewrite* dom_kinds_open_vars.
+        disjoint_solve.
+      intuition.
+        intro; intros.
+        apply H3.
+        rewrite map_concat.
+        apply* binds_concat_ok.
+        rewrite <- map_concat.
+        apply* ok_map0.
+      replace (map (sch_subst S) E)
+        with (map (sch_subst S) (map (sch_subst S0) E)).
+      destruct* (unify_type _ _ HI).
+        simpl; intros.
+        destruct* H1.
+        inversions H1; clear H1.
+        split*.
+        unfold sch_open_vars.
+        refine (proj1 (HSE _ _ R1 x _)). auto.
+      use (unify_types _ _ _ HI HS0).
+      rewrite* <- (H5 (sch_open_vars s x) T).
+      rewrite* <- (typ_subst_extend _ _ _ HS0 HI).
+      rewrite* sch_subst_open_vars.
+      apply* typing_typ_well_subst.
+        apply* kenv_ok_map.
+      unfold sch_open_vars, typ_open_vars.
+      fold (sch_open (sch_subst S0 s) (typ_fvars x)).
+      apply* typing_var.
+        apply* kenv_ok_map.
+      split.
+        unfold sch_arity. simpl. rewrite map_length. fold (sch_arity s).
+        rewrite (fresh_length _ _ _ f). apply types_typ_fvars.
+      split. apply* sch_subst_type. apply (HSE _ _ R1).
+
+Qed.
+         
+End Mk2.
+End MkInfer.
